Formalization of bitwise operators (#423)
* Fromalize integerToByteString

* feat: integerToByteString formalization - in progress...

* feat: integerToByteString formalization - in progress...

* eat: integerToByteString formalization - in progress...

* feat: implement bitwise operations

* fix: bitwise operations - self-review

* doc: document the desgin choice of the bitwise operation implementations

PlutusCore/Bitwise/Basic.lean
@@ -1,29 +1,252 @@
-import PlutusCore.ByteString
 import PlutusCore.Integer
 
 namespace PlutusCore.Bitwise
-open PlutusCore.ByteString PlutusCore.Integer
+open PlutusCore.Integer
 
 /-! ## Formalisation for PlutusCore Logical and Bitwise builtin functions on ByteString. -/
 
-namespace PlutusCore.BitwiseInternal
+/- Intead of recreating the Haskell implementation, the design choice was to
+   implement the functions in Lean in a way that the observable behavior (responses)
+   are the same. This means that successful results are the same and for errors,
+   the same error messages are returned in a Left case; the difference is that error
+   "traces" are not generated. -/
 
--- TODO: integerToByteString : Bool → Integer → Integer → Except String ByteString
--- TODO: byteStringToInteger : Bool → ByteString → Integer
--- TODO: andByteString : Bool → ByteString → ByteString → ByteString
--- TODO: orByteString : Bool → ByteString → ByteSgtring → ByteString
--- TODO: xorByteString : Bool → ByteString → ByteString → ByteString
--- TODO: complementByteString : ByteString → ByteString
--- TODO: shiftByteString : ByteString → Integer → ByteString
--- TODO: rotateByteString : ByteString → Integer → ByteString
--- TODO: countSetBits : ByteString → Integer
--- TODO: findFirstSetBit : ByteString → Integer
--- TODO: readBit : ByteString → Integer → Except String Bool
--- TODO: writeBits : ByteString → List Integer → Bool → Except String ByteString
--- TODO: replicateByte : Integer → Integer → Except String ByteString
+namespace BitwiseInternal
 
-end PlutusCore.BitwiseInternal
--- TODO: add export list
+/-- The maximum length that `integerToByteString` and `replicateByte` can handle. -/
+@[simp] def maxOutputLength     : Nat := 8192
+@[simp] def maxOutputBitsLength : Nat := 8 * maxOutputLength
+
+/-- Calculates the base-2 logarithm of Integers, returns 0 for negative values. -/
+def integerLog2 : Integer → Nat
+  | .negSucc _ => 0
+  | .ofNat   n => Nat.log2 n
+
+/-- Calculates the "width" of a number in bytes. -/
+def integerWidth : Nat → Nat
+  | 0 => 0
+  | n => Nat.log2 n / 8 + 1
+
+/-- Calculates the big-endian representation of a natural number with maximal byte width.
+    Tail recursive version, uses accumulator for the calculation. -/
+def itobs_be_loop : Nat → List Char → Nat → Except String (List Char)
+  | .succ p, a, n => itobs_be_loop p (Char.ofNat (n % 256) :: a) (n / 256)
+  | .zero  , a, 0 => pure a
+  | .zero  , _, _ => throw "integerToByteString: cannot represent Integer in given number of bytes"
+
+/-- Converts a non-negative integer to a bytestring.
+    ```
+    (e, w, n) → itobs_le (w, n), if e = false
+                 itobs_be (w, n), if e = true
+
+    Let 𝑛 = ∑_(𝑖=0)^(𝑁−1) 𝑎_𝑖 * 256 ^ 𝑖
+      with 𝑁 ≥ 1, 𝑎_𝑖 ∈ [0..256] for 0 ≤ 𝑖 ≤ 𝑁 − 1 and 𝑎_(𝑁−1) ≠ 0
+
+    itobs_le (𝑤, 𝑛) = itobs_be (w, n) :=
+        ×,  if 𝑛 < 0 or 𝑛 ≥ 265536
+        ×,  if 𝑤 < 0 or 𝑤 > 8192
+        [], if 𝑛 = 0 and 0 ≤ 𝑤 ≤ 8192
+
+    itobs_le (w, n) :=
+      [𝑎_0, … , 𝑎_(𝑁−1)], if 𝑤 = 0
+      [𝑏_0, … , 𝑏_(𝑤−1)], if 𝑤 > 0 and 𝑁 ≤ 𝑤,
+      ×                  , if 𝑤 > 0 and 𝑁 > 𝑤
+        where
+          b_i := 𝑎_𝑖, if 𝑖 ≤ 𝑁 − 1
+                 0  , if 𝑖 ≥ 𝑁
+
+    𝗍𝗈𝖻𝗌_be(𝑤, 𝑛) :=
+      [𝑎_(𝑁−1), … , 𝑎_0], if 𝑤 = 0
+      [𝑏_0, … , 𝑏_(𝑤−1)], if 𝑤 > 0 and 𝑁 ≤ 𝑤
+      ×                  , if 𝑤 > 0 and 𝑁 > 𝑤
+        where
+          b_i := 0        , if 𝑖 ≤ 𝑤 − 1 − 𝑁
+                 𝑎_(𝑤−1−𝑖), if 𝑖 ≥ 𝑤 − 𝑁
+    ```
+-/
+@[simp]
+def integerToByteString (e : Bool) (w n : Integer) : Except String String :=
+       if w < 0                                       then throw "integerToByteString: negative length argument"
+  else if w > maxOutputLength                         then throw s!"integerToByteString: requested length is too long (maximum is {maxOutputLength} bytes)"
+  else if w = 0 ∧ integerLog2 n ≥ maxOutputBitsLength then throw s!"integerToByteString: input too long (maximum is 2^{maxOutputBitsLength}-1)"
+  else if n < 0                                       then throw "integerToByteString: cannot convert negative Integer"
+  else do
+    let r ← match w, n with
+             | 0        , 0         => pure []
+             | 0        , .ofNat n' => itobs_be_loop (integerWidth n') [] n'
+             | .ofNat w', .ofNat n' => itobs_be_loop w'                [] n'
+             | _        , _         => unreachable!
+    if e then pure ⟨r⟩
+         else pure ⟨r.reverse⟩
+
+/-- Reconstructs a natural number from it's big-endian representation.
+    Tail recursive version, uses accumulator for the calculation. -/
+def bstoi_be_loop : List Char → Nat → Nat
+  | []    , acc => acc
+  | h :: t, acc => bstoi_be_loop t (acc * 256 + (Char.toNat h))
+
+/-- The `byteStringToInteger` function converts bytestrings to non-negative integers. -/
+def byteStringToInteger (e : Bool) (s : String) : Integer :=
+  if e then .ofNat (bstoi_be_loop s.data         0)
+       else .ofNat (bstoi_be_loop s.data.reverse 0)
+
+/-- Truncates `b` by `k` number of characters (bytes). -/
+def trunc (b : String) (k : Nat) : String := String.dropRight b k
+
+/-- Extends `b` by `k` number of characters (bytes) of full 1 bits in case `ones` is true (zeroes otherwise). -/
+def ext (b : String) (k : Nat) (ones : Bool) : String := String.pushn b (if ones then '\xFF' else '\x00') k
+
+/-- Helper function that truncates or extends a string as necessary. -/
+def truncateOrExtend : Bool → String → Nat → Bool → String
+  | false, s, n, _    => let m := String.length s; let l := Nat.min m n; trunc s (m - l)
+  | true , s, n, ones => let m := String.length s; let l := Nat.max m n; ext   s (l - m) ones
+
+/-- Helper function to extend a binary bitwise operation to Strings.
+    Extends the shorter string if `e` is true, otherwise truncates the longer. -/
+def byteStringOp (op : Nat → Nat → Nat) (ones e : Bool) (b c : String) : String :=
+  let m   := String.length b
+  let n   := String.length c
+  let b'  := truncateOrExtend e b n ones
+  let c'  := truncateOrExtend e c m ones
+  let b'' := (·.toUInt8.toNat) <$> String.toList b'
+  let c'' := (·.toUInt8.toNat) <$> String.toList c'
+  let r   := Function.uncurry op <$> List.zip b'' c''
+  ⟨Char.ofNat <$> r⟩
+
+/-- Performs bitwise `and` on bytestrings, extending the lengths if the bool argument is true. -/
+def andByteString : Bool → String → String → String := byteStringOp (· &&& ·) true
+/-- Performs bitwise `or` on bytestrings, extending the lengths if the bool argument is true. -/
+def  orByteString : Bool → String → String → String := byteStringOp (· ||| ·) false
+/-- Performs bitwise `xor` on bytestrings, extending the lengths if the bool argument is true. -/
+def xorByteString : Bool → String → String → String := byteStringOp (· ^^^ ·) false
+
+/-- Performs bitwise complementer calculation on the input bytestring. -/
+def complementByteString (b : String) : String := xorByteString false (String.map (λ _ => '\xFF') b) b
+
+/- Generates a bit sequence from a bytestring.
+   Tail recursive version, uses accumulator for the calculation. -/
+def bitSequenceFromByteString : List Char → List Bool → List Bool
+  | []    , acc => acc
+  | c :: t, acc =>
+      let b   := c |> Char.toUInt8 |> UInt8.toBitVec
+      let bcc := [b.getLsb 7, b.getLsb 6, b.getLsb 5, b.getLsb 4, b.getLsb 3, b.getLsb 2, b.getLsb 1, b.getLsb 0]
+      bitSequenceFromByteString t (acc ++ bcc)
+
+/-- Reconstruct a Natural number from it's base-2 big-endian representation.
+    Tail recursive version, uses accumulator for the calculation. -/
+def reconstructNat : List Bool → Nat → Nat
+  | false :: t, acc => reconstructNat t (2 * acc)
+  | true  :: t, acc => reconstructNat t (2 * acc + 1)
+  | []        , acc => acc
+
+/-- Generates a bytestring from a bit sequence.
+    Tail recursive version, uses accumulator for the calculation. -/
+def bitSequenceToByteString : List Bool → List Char → Option (List Char)
+  | b₇ :: b₆ :: b₅ :: b₄ :: b₃ :: b₂ :: b₁ :: b₀ :: t, acc =>
+      bitSequenceToByteString t (Char.ofNat (reconstructNat [b₇, b₆, b₅, b₄, b₃, b₂, b₁, b₀] 0) :: acc)
+  | []                                               , acc => .some (List.reverse acc)
+  | _                                                , _   => .none
+
+/-- Shifts the bits of `s`
+    - `k` places to the left if `k ≥ 0`
+    - `k` places to the right if `k < 0` -/
+def shiftByteString (s : String) (k : Integer) : String :=
+  let bs  := bitSequenceFromByteString s.data []
+  let l   := List.length bs
+  let bs' := match k with
+             | .ofNat n   => if n < l then List.drop n (bs ++ List.replicate n false)
+                                      else List.replicate l false
+             | .negSucc n => if n + 1 < l then List.take l (List.replicate (n + 1) false ++ bs)
+                                          else List.replicate l false
+  match bitSequenceToByteString bs' [] with
+  | .some x => ⟨x⟩
+  | _       => unreachable!
+
+/-- Rotates the bits of `s`
+    - `k` places to the left if `k ≥ 0`
+    - `k` places to the right if `k < 0` -/
+def rotateByteString (s : String) (k : Integer) : String :=
+  let bs  := bitSequenceFromByteString s.data []
+  let l   := List.length bs
+  let bs' := match k with
+             | .ofNat n   => List.take l (List.drop (n % l)             (bs ++ bs))
+             | .negSucc n => List.take l (List.drop (l - ((n + 1) % l)) (bs ++ bs))
+  match bitSequenceToByteString bs' [] with
+  | .some x => ⟨x⟩
+  | _       => unreachable!
+
+/-- Counts the number of set bits (1) in `s`. -/
+def countSetBits (s : String) : Integer :=
+  List.count true (bitSequenceFromByteString s.data [])
+
+/-- Finds the index of the first set bit (1) in a bytestring from the _right_.
+    Returns -1, if no bits are set. -/
+def findFirstSetBit (s : String) : Integer :=
+  match bitSequenceFromByteString s.data [] |> List.reverse |> List.findIdx? (·) with
+  | .some i => .ofNat i
+  | .none   => -1
+
+/-- Returns the value of the nth bit in the bytestring.
+    Bits are indexed from the _right_. -/
+def readBit : String → Integer → Except String Bool
+  | _, .negSucc _ => throw "readBit: index out of bounds"
+  | s, .ofNat   i =>
+      let len := String.length s
+      if 8 * len ≤ i then throw "readBit: index out of bounds"
+      else
+        let bigIx      := i / 8
+        have h : 8 > 0 := by simp
+        let littleIx   := ⟨i % 8, Nat.mod_lt i h⟩
+        let flipIx     := len - bigIx - 1
+        pure (BitVec.getLsb (s.data[flipIx]! |> Char.toUInt8 |> UInt8.toBitVec) littleIx)
+
+def writeBit : String → Integer → Bool → Except String String
+  | _, .negSucc _, _ => throw "writeBits: index out of bounds"
+  | s, .ofNat   i, x =>
+      let len := String.length s
+      if 8 * len ≤ i then throw "writeBits: index out of bounds"
+      else
+        let bigIx    := i / 8
+        let littleIx := i % 8
+        let flipIx   := len - bigIx - 1
+        let bs       := s.data[flipIx]! |> Char.toUInt8 |> UInt8.toNat
+        let mask     := 0x1 <<< littleIx
+        let bs'      := if x then bs ||| mask
+                               else bs &&& (mask ^^^ 0xFF)
+        pure ⟨List.set s.data flipIx (bs' |> Char.ofNat)⟩
+
+/-- Writes the value of the list of bits in the bytestring.
+    Bits are indexed from the _right_. -/
+def writeBits : String → List Integer → Bool → Except String String
+  | s, h :: t, x => do writeBits (←writeBit s h x) t x
+  | s, []    , _ => pure s
+
+/-- Creates a bytestring by repeating the provided value n times. -/
+def replicateByte : Integer → Integer → Except String String
+  | .negSucc _, _          => throw "replicateByte: negative length requested"
+  | _         , .negSucc _ => throw "replicateByte: negative byte requested"
+  | .ofNat   l, .ofNat   b =>
+           if maxOutputLength < l then throw s!"replicateByte: requested length is too long (maximum is {maxOutputLength} bytes)"
+      else if 255             < b then throw "replicateByte: requested byte is out of range (maximum is 255)"
+      else pure ⟨List.replicate l (Char.ofNat b)⟩
+
+end BitwiseInternal
+
+export BitwiseInternal
+  ( -- builtin functions
+    integerToByteString
+    byteStringToInteger
+    andByteString
+    orByteString
+    xorByteString
+    complementByteString
+    shiftByteString
+    rotateByteString
+    countSetBits
+    findFirstSetBit
+    readBit
+    writeBits
+    replicateByte
+  )
 
 end PlutusCore.Bitwise
-
